뭐지. 왜 F# 빌드에서 말썽이야?

src/study/Nemonuri.Study.CSharpSyntaxRewriter2.Modifier/Nemonuri.StratifiedNode.NodeTheory.Child.fst
@@ -35,6 +35,7 @@ let get_child_node_index
   : Tot (child_node_index parent)
   = index_of parent.children cn
 
+(*
 let child_node_func
   (t:eqtype) (t2:Type) =
     (#parent_level:pos) ->
@@ -42,13 +43,21 @@ let child_node_func
     (#child_level:pos) ->
     (cn:(child_node parent child_level)) ->
     Tot t2
+*)
+
+let child_node_func
+  (t:eqtype) (t2:Type)
+  (#parent_level:pos) (parent:stratified_node t parent_level) =
+    (#child_level:pos) ->
+    (cn:(child_node parent child_level)) ->
+    Tot t2
+
+let child_node_func_builder (t:eqtype) (t2:Type) =
+  (#parent_level:pos) -> 
+  (parent:stratified_node t parent_level) ->
+  Tot (child_node_func t t2 parent)
 
 (*
-let parent_bound_child_node_func
-  (t:eqtype) (t2:Type)
-  (#parent_level:pos) (parent:stratified_node t parent_level)
-  = (refined_stratified_node_func t t2 (is_child parent))
-
 let bound_parent
   (#t:eqtype) (#t2:Type) (#parent_level:pos) (parent:stratified_node t parent_level)
   (cnf:child_node_func t t2)
@@ -82,9 +91,17 @@ let child_node_and_index_func
     Tot t2
 *)
 
-let child_node_predicate (t:eqtype) =
-  child_node_func t bool
+let child_node_predicate
+  (t:eqtype)
+  (#parent_level:pos) (parent:stratified_node t parent_level) =
+  child_node_func t bool #parent_level parent
 
+let child_node_predicate_builder (t:eqtype) =
+  (#parent_level:pos) -> 
+  (parent:stratified_node t parent_level) ->
+  Tot (child_node_predicate t parent)
+
+(*
 let refined_child_node_func
   (t:eqtype) (t2:Type) (predicate:child_node_predicate t) =
   (#parent_level:pos) ->
@@ -95,6 +112,7 @@ let refined_child_node_func
 
 let refined_child_node_predicate (t:eqtype) (predicate:child_node_predicate t) =
   refined_child_node_func t bool predicate
+*)
 
 (*
 let convert_stratified_node_predicate_to_child_node_predicate
@@ -120,7 +138,7 @@ private let rec select_in_children_core
   (#children_mlv:nat)
   (subchildren:stratified_node_list t children_mlv{ is_subchildren parent subchildren })
   (#t2:Type) 
-  (selector:refined_child_node_func t t2 (fun parent1 child1 -> (is_equal_node parent parent1) && (is_child parent1 child1)))
+  (selector:child_node_func t t2 parent)
   : Tot (x:(list t2){ L.length x = get_length subchildren }) 
         (decreases subchildren)
   = if is_empty subchildren then 
@@ -129,13 +147,13 @@ private let rec select_in_children_core
       (
         lemma_for_subchildren parent subchildren;
         let hd = get_hd subchildren in
-        (selector parent hd)::
+        (selector hd)::
         (select_in_children_core parent (get_tl subchildren) selector)
       )
 
 let select_in_children
   (#t:eqtype) (#lv:pos) (parent:stratified_node t lv) (#t2:Type)
-  (selector:refined_child_node_func t t2 (fun parent1 child1 -> (is_equal_node parent parent1) && (is_child parent1 child1)))
+  (selector:child_node_func t t2 parent)
   : Tot (x:(list t2){ L.length x = get_length parent.children })
   = select_in_children_core parent parent.children selector
 
@@ -143,14 +161,14 @@ private let rec exists_in_children_core
   (#t:eqtype) (#lv:pos) (parent:stratified_node t lv) 
   (#children_mlv:nat)
   (subchildren:stratified_node_list t children_mlv{ is_subchildren parent subchildren })
-  (predicate:refined_child_node_predicate t (fun parent1 child1 -> (is_equal_node parent parent1) && (is_child parent1 child1)))
+  (predicate:child_node_predicate t parent)
   : Tot bool (decreases subchildren)
   = if is_empty subchildren then 
       false
     else
       (
         lemma_for_subchildren parent subchildren;
-        if predicate parent (get_hd subchildren) then 
+        if predicate (get_hd subchildren) then 
           true
         else 
           exists_in_children_core parent (get_tl subchildren) predicate
@@ -158,7 +176,7 @@ private let rec exists_in_children_core
 
 let exists_in_children
   (#t:eqtype) (#lv:pos) (parent:stratified_node t lv)
-  (predicate:refined_child_node_predicate t (fun parent1 child1 -> (is_equal_node parent parent1) && (is_child parent1 child1)))
+  (predicate:child_node_predicate t parent)
   : Tot bool
   = exists_in_children_core parent parent.children predicate
 
