src/study/Nemonuri.Study.CSharpSyntaxRewriter2.Modifier/Nemonuri.StratifiedNode.IndexTheory.Base.fst
@@ -68,7 +68,7 @@ private let rec try_get_index_of_child_from_predicate_core
   (#t:eqtype) (#lv:pos) (parent:stratified_node t lv) 
   (#children_mlv:nat)
   (subchildren:stratified_node_list t children_mlv{ is_subchildren parent subchildren })
-  (predicate:refined_child_node_predicate t (fun parent1 child1 -> (is_equal_node parent parent1) && (is_child parent1 child1)))
+  (predicate:child_node_predicate t parent)
   : Tot (option (child_node_index parent)) 
         (decreases subchildren)
   = if is_empty subchildren then 
@@ -76,7 +76,7 @@ private let rec try_get_index_of_child_from_predicate_core
     else
       (
         lemma_for_subchildren parent subchildren;
-        if predicate parent (get_hd subchildren) then 
+        if predicate (get_hd subchildren) then 
           Some ((get_children_length parent) - (get_length subchildren))
         else 
           try_get_index_of_child_from_predicate_core parent (get_tl subchildren) predicate
@@ -84,47 +84,43 @@ private let rec try_get_index_of_child_from_predicate_core
 
 let try_get_index_of_child_from_predicate
   (#t:eqtype) (#lv:pos) (parent:stratified_node t lv)
-  (predicate:refined_child_node_predicate t (fun parent1 child1 -> (is_equal_node parent parent1) && (is_child parent1 child1)))
+  (predicate:child_node_predicate t parent)
   : Tot (option (child_node_index parent)) 
   = try_get_index_of_child_from_predicate_core parent parent.children predicate
 
-#push-options "--query_stats"
-let rec try_get_indexes_of_descendant_or_self_from_predicate_core
+private let rec try_get_indexes_of_descendant_or_self_from_predicate_core
   (#t:eqtype) (#lv:pos) (parent:stratified_node t lv) (parent_indexes:stratified_node_indexes)
-  (predicate:refined_child_node_predicate t (fun parent1 child1 -> (is_equal_node parent parent1) && (is_child parent1 child1)))
+  (predicate_builder:child_node_predicate_builder t)
   : Tot (option (stratified_node_indexes)) 
         (decreases lv)
-  = match (try_get_index_of_child_from_predicate parent predicate) with
-  | Some v1 -> Some (add_index parent_indexes v1)
-  | None -> 
+  = match (try_get_index_of_child_from_predicate #t #lv parent (predicate_builder parent)) with
+    | Some v1 -> Some (add_index parent_indexes v1)
+    | None -> 
     let v2 =
       select_in_children parent (
-        fun psn csn -> (
-          //lemma_child_node_level_is_lower_than_parent psn csn;
-          assert (lv > (get_level csn));
+        fun csn -> (
           let cni = get_child_node_index csn in
           let new_parent_indexes = add_index parent_indexes cni in
-          try_get_indexes_of_descendant_or_self_from_predicate_core csn new_parent_indexes predicate
+          try_get_indexes_of_descendant_or_self_from_predicate_core csn new_parent_indexes predicate_builder
         )
       ) in
     let v3 = L.find (Some?) v2 in
     match v3 with
     | None -> None
     | Some v4 -> v4
-#pop-options
-      
-      
-//let cnp = convert_stratified_node_predicate_to_child_node_predicate predicate sn in
 
-(*
-let rec try_get_indexes_of_descendant_or_self_from_predicate
+
+let try_get_indexes_of_descendant_or_self_from_predicate
   (#t:eqtype) (#lv:pos) (root:stratified_node t lv)
   (predicate:stratified_node_predicate t)
   : Tot (option (stratified_node_indexes)) 
   = if (predicate root) then
       Some empty_stratified_node_indexes
     else
-*)
+      try_get_indexes_of_descendant_or_self_from_predicate_core root empty_stratified_node_indexes
+        (fun (#parent_level:pos) (parent:stratified_node t parent_level) ->
+          (fun (#child_level:pos) (child:(child_node parent child_level)) -> predicate child)
+        )
 
 (*
   = match (if (predicate parent) then (Some empty_stratified_node_indexes) else None) with
