src/study/Nemonuri.Study.CSharpSyntaxRewriter2.Modifier/Nemonuri.StratifiedNode.NodeTheory.Descendant.fst
@@ -27,7 +27,7 @@ let rec get_count
     else 
       sum_for_get_count #t #lv #sn (
         select_in_children sn (
-          fun psn csn -> (
+          fun csn -> (
             //lemma_child_node_level_is_lower_than_parent psn csn;
             get_count csn <: nat
           )
@@ -42,7 +42,7 @@ let rec exists_in_descendant_or_self
       false
     else
       exists_in_children sn (
-        fun psn csn -> (
+        fun csn -> (
           //lemma_child_node_level_is_lower_than_parent psn csn;
           exists_in_descendant_or_self csn predicate
         )
